ntruplus/proof/768/ref/poly_tobytes/NTRUPlus768PolyToBytesAlgebra.ec
@@ -1,0 +1,355 @@
+require import AllCore IntDiv Ring StdOrder.
+from Jasmin require import JWord JModel_x86.
+
+require import Array768 Array1152.
+require import NTRUPlus768BasemulAlgebra.
+require import NTRUPlus768PolyToBytesProof.
+
+import Ring.IntID IntOrder.
+
+op poly_tobytes_input_qrange (p : W16.t Array768.t) : bool =
+  forall j, 0 <= j < 768 => -q <= coeff p.[j] < q.
+
+op canonical_coeff (w : W16.t) : int =
+  if coeff w < 0 then coeff w + q else coeff w.
+
+op poly_tobytes_byte0_int (p : W16.t Array768.t) (i : int) : int =
+  canonical_coeff p.[2 * i] %% 256.
+
+op poly_tobytes_byte1_int (p : W16.t Array768.t) (i : int) : int =
+  canonical_coeff p.[2 * i] %/ 256 + 16 * (canonical_coeff p.[2 * i + 1] %% 16).
+
+op poly_tobytes_byte2_int (p : W16.t Array768.t) (i : int) : int =
+  canonical_coeff p.[2 * i + 1] %/ 16.
+
+op poly_tobytes_byte_at (p : W16.t Array768.t) (j : int) : W8.t =
+  if j %% 3 = 0 then
+    W8.of_int (poly_tobytes_byte0_int p (j %/ 3))
+  else if j %% 3 = 1 then
+    W8.of_int (poly_tobytes_byte1_int p (j %/ 3))
+  else
+    W8.of_int (poly_tobytes_byte2_int p (j %/ 3)).
+
+op poly_tobytes_spec (p : W16.t Array768.t) : W8.t Array1152.t =
+  Array1152.init (fun j => poly_tobytes_byte_at p j).
+
+op poly_tobytes_canonical_spec (p : W16.t Array768.t) : W16.t Array768.t =
+  Array768.init (fun j => W16.of_int (canonical_coeff p.[j])).
+
+op poly_frombytes_even_int (a : W8.t Array1152.t) (i : int) : int =
+  W8.to_uint a.[3 * i] + 256 * (W8.to_uint a.[3 * i + 1] %% 16).
+
+op poly_frombytes_odd_int (a : W8.t Array1152.t) (i : int) : int =
+  W8.to_uint a.[3 * i + 1] %/ 16 + 16 * W8.to_uint a.[3 * i + 2].
+
+op poly_frombytes_int (a : W8.t Array1152.t) (j : int) : int =
+  if j %% 2 = 0 then
+    poly_frombytes_even_int a (j %/ 2)
+  else
+    poly_frombytes_odd_int a (j %/ 2).
+
+op poly_frombytes_spec (a : W8.t Array1152.t) : W16.t Array768.t =
+  Array768.init (fun j => W16.of_int (poly_frombytes_int a j)).
+
+lemma poly_tobytes_procedure_input_qrangeE
+    (p : W16.t Array768.t) :
+  NTRUPlus768PolyToBytesProof.poly_tobytes_input_qrange p =
+  poly_tobytes_input_qrange p.
+proof.
+  rewrite /NTRUPlus768PolyToBytesProof.poly_tobytes_input_qrange
+    /poly_tobytes_input_qrange.
+  done.
+qed.
+
+lemma poly_tobytes_procedure_specE (p : W16.t Array768.t) :
+  NTRUPlus768PolyToBytesProof.poly_tobytes_spec p = poly_tobytes_spec p.
+proof.
+  rewrite /NTRUPlus768PolyToBytesProof.poly_tobytes_spec /poly_tobytes_spec
+    /NTRUPlus768PolyToBytesProof.poly_tobytes_byte_at /poly_tobytes_byte_at
+    /NTRUPlus768PolyToBytesProof.poly_tobytes_byte0_int
+    /poly_tobytes_byte0_int
+    /NTRUPlus768PolyToBytesProof.poly_tobytes_byte1_int
+    /poly_tobytes_byte1_int
+    /NTRUPlus768PolyToBytesProof.poly_tobytes_byte2_int
+    /poly_tobytes_byte2_int
+    /NTRUPlus768PolyToBytesProof.canonical_coeff /canonical_coeff.
+  done.
+qed.
+
+lemma coeff_of_word_small (x : int) :
+  W16.min_sint <= x <= W16.max_sint =>
+  coeff (W16.of_int x) = x.
+proof.
+  move=> Hx.
+  rewrite /coeff.
+  exact (W16.to_sintK_small x Hx).
+qed.
+
+lemma canonical_coeff_range (w : W16.t) :
+  -q <= coeff w < q =>
+  0 <= canonical_coeff w < q.
+proof.
+  move=> Hw.
+  rewrite /canonical_coeff.
+  case (coeff w < 0).
+  + move=> Hneg.
+    rewrite /q /=.
+    smt().
+  move=> Hnonneg.
+  rewrite /q /=.
+  smt().
+qed.
+
+lemma poly_tobytes_canonical_coeff_range
+    (p : W16.t Array768.t) (j : int) :
+  poly_tobytes_input_qrange p =>
+  0 <= j < 768 =>
+  0 <= canonical_coeff p.[j] < q.
+proof.
+  move=> Hp Hj.
+  exact (canonical_coeff_range p.[j] (Hp j Hj)).
+qed.
+
+lemma poly_tobytes_byte0_range (p : W16.t Array768.t) (i : int) :
+  poly_tobytes_input_qrange p =>
+  0 <= i < 384 =>
+  0 <= poly_tobytes_byte0_int p i < 256.
+proof.
+  move=> Hp Hi.
+  have Hcanon := poly_tobytes_canonical_coeff_range p (2 * i) Hp _.
+  + smt().
+  rewrite /poly_tobytes_byte0_int.
+  smt().
+qed.
+
+lemma poly_tobytes_byte1_range (p : W16.t Array768.t) (i : int) :
+  poly_tobytes_input_qrange p =>
+  0 <= i < 384 =>
+  0 <= poly_tobytes_byte1_int p i < 256.
+proof.
+  move=> Hp Hi.
+  have Hc0 := poly_tobytes_canonical_coeff_range p (2 * i) Hp _.
+  + smt().
+  have Hc1 := poly_tobytes_canonical_coeff_range p (2 * i + 1) Hp _.
+  + smt().
+  rewrite /poly_tobytes_byte1_int.
+  have Hdiv : 0 <= canonical_coeff p.[2 * i] %/ 256 < 16 by smt().
+  have Hmod : 0 <= canonical_coeff p.[2 * i + 1] %% 16 < 16 by smt().
+  smt().
+qed.
+
+lemma poly_tobytes_byte2_range (p : W16.t Array768.t) (i : int) :
+  poly_tobytes_input_qrange p =>
+  0 <= i < 384 =>
+  0 <= poly_tobytes_byte2_int p i < 256.
+proof.
+  move=> Hp Hi.
+  have Hcanon := poly_tobytes_canonical_coeff_range p (2 * i + 1) Hp _.
+  + smt().
+  rewrite /poly_tobytes_byte2_int.
+  smt().
+qed.
+
+lemma poly_tobytes_spec_byte0E (p : W16.t Array768.t) (i : int) :
+  0 <= i < 384 =>
+  (poly_tobytes_spec p).[3 * i] = W8.of_int (poly_tobytes_byte0_int p i).
+proof.
+  move=> Hi.
+  rewrite /poly_tobytes_spec Array1152.initiE 1:/# /poly_tobytes_byte_at.
+  smt().
+qed.
+
+lemma poly_tobytes_spec_byte1E (p : W16.t Array768.t) (i : int) :
+  0 <= i < 384 =>
+  (poly_tobytes_spec p).[3 * i + 1] = W8.of_int (poly_tobytes_byte1_int p i).
+proof.
+  move=> Hi.
+  rewrite /poly_tobytes_spec Array1152.initiE 1:/# /poly_tobytes_byte_at.
+  smt().
+qed.
+
+lemma poly_tobytes_spec_byte2E (p : W16.t Array768.t) (i : int) :
+  0 <= i < 384 =>
+  (poly_tobytes_spec p).[3 * i + 2] = W8.of_int (poly_tobytes_byte2_int p i).
+proof.
+  move=> Hi.
+  rewrite /poly_tobytes_spec Array1152.initiE 1:/# /poly_tobytes_byte_at.
+  smt().
+qed.
+
+lemma poly_tobytes_canonical_spec_coeff
+    (p : W16.t Array768.t) (j : int) :
+  poly_tobytes_input_qrange p =>
+  0 <= j < 768 =>
+  coeff (poly_tobytes_canonical_spec p).[j] = canonical_coeff p.[j].
+proof.
+  move=> Hp Hj.
+  rewrite /poly_tobytes_canonical_spec Array768.initiE 1:/#.
+  apply coeff_of_word_small.
+  have Hrange := poly_tobytes_canonical_coeff_range p j Hp Hj.
+  rewrite /q /= in Hrange.
+  smt().
+qed.
+
+lemma canonical_coeff_mod_q (w : W16.t) :
+  -q <= coeff w < q =>
+  canonical_coeff w %% q = coeff w %% q.
+proof.
+  move=> Hw.
+  rewrite /canonical_coeff.
+  case (coeff w < 0).
+  + move=> Hneg.
+    rewrite /q /=.
+    smt().
+  move=> Hnonneg.
+  by [].
+qed.
+
+lemma poly_tobytes_canonical_spec_mod_q
+    (p : W16.t Array768.t) (j : int) :
+  poly_tobytes_input_qrange p =>
+  0 <= j < 768 =>
+  coeff (poly_tobytes_canonical_spec p).[j] %% q = coeff p.[j] %% q.
+proof.
+  move=> Hp Hj.
+  have Hcoeff :
+      coeff (poly_tobytes_canonical_spec p).[j] = canonical_coeff p.[j]
+    by exact (poly_tobytes_canonical_spec_coeff p j Hp Hj).
+  rewrite Hcoeff.
+  exact (canonical_coeff_mod_q p.[j] (Hp j Hj)).
+qed.
+
+lemma poly_frombytes_spec_coeff_uint (a : W8.t Array1152.t) (j : int) :
+  0 <= j < 768 =>
+  W16.to_uint (poly_frombytes_spec a).[j] = poly_frombytes_int a j.
+proof.
+  move=> Hj.
+  rewrite /poly_frombytes_spec Array768.initiE 1:/# W16.of_uintK.
+  rewrite /poly_frombytes_int.
+  case (j %% 2 = 0).
+  + move=> _.
+    rewrite /poly_frombytes_even_int.
+    have Hb0 := W8.to_uint_cmp a.[3 * (j %/ 2)].
+    have Hb1 := W8.to_uint_cmp a.[3 * (j %/ 2) + 1].
+    have H8e : W8.modulus = 256 by done.
+    have H16e : W16.modulus = 65536 by done.
+    rewrite (modz_small _ 65536).
+    smt(modz_cmp).
+    trivial.
+  move=> _.
+  rewrite /poly_frombytes_odd_int.
+  have Hb1 := W8.to_uint_cmp a.[3 * (j %/ 2) + 1].
+  have Hb2 := W8.to_uint_cmp a.[3 * (j %/ 2) + 2].
+  have H8o : W8.modulus = 256 by done.
+  have H16o : W16.modulus = 65536 by done.
+  rewrite (modz_small _ 65536).
+  smt(modz_cmp).
+  trivial.
+qed.
+
+lemma poly_frombytes_poly_tobytes_roundtrip
+    (p : W16.t Array768.t) :
+  poly_tobytes_input_qrange p =>
+  poly_frombytes_spec (poly_tobytes_spec p) = poly_tobytes_canonical_spec p.
+proof.
+  move=> Hp.
+  apply Array768.tP => j Hj.
+  apply W16.to_uint_eq.
+  rewrite poly_frombytes_spec_coeff_uint 1:Hj.
+  rewrite /poly_tobytes_canonical_spec Array768.initiE 1:Hj W16.of_uintK.
+  have Hcanon := poly_tobytes_canonical_coeff_range p j Hp Hj.
+  have H16 : W16.modulus = 65536 by done.
+  rewrite (modz_small _ 65536).
+  + smt().
+  rewrite /poly_frombytes_int.
+  case (j %% 2 = 0).
+  + move=> Heven.
+    have Hi : 0 <= j %/ 2 < 384 by smt().
+    rewrite /poly_frombytes_even_int.
+    rewrite poly_tobytes_spec_byte0E 1:/# poly_tobytes_spec_byte1E 1:/#.
+    rewrite W8.of_uintK.
+    - rewrite W8.of_uintK.
+      * rewrite /poly_tobytes_byte0_int /poly_tobytes_byte1_int.
+        have Hc0 := poly_tobytes_canonical_coeff_range p j Hp Hj.
+        have Hc1 := poly_tobytes_canonical_coeff_range p (j + 1) Hp _.
+        + smt().
+        have Hmod : 0 <= canonical_coeff p.[j + 1] %% 16 < 16 by smt().
+        have Hdiv : 0 <= canonical_coeff p.[j] %/ 256 < 16 by smt().
+        smt().
+  move=> Hodd.
+  have Hi : 0 <= j %/ 2 < 384 by smt().
+  rewrite /poly_frombytes_odd_int.
+  rewrite poly_tobytes_spec_byte1E 1:/# poly_tobytes_spec_byte2E 1:/#.
+  rewrite W8.of_uintK.
+  + rewrite W8.of_uintK.
+    - rewrite /poly_tobytes_byte1_int /poly_tobytes_byte2_int.
+      have Hc0 := poly_tobytes_canonical_coeff_range p (j - 1) Hp _.
+      + smt().
+      have Hc1 := poly_tobytes_canonical_coeff_range p j Hp Hj.
+      have Hmid : 0 <= canonical_coeff p.[j - 1] %/ 256 < 16 by smt().
+      have Hhi : 0 <= canonical_coeff p.[j] %/ 16 < 256 by smt().
+      have Hmod : 0 <= canonical_coeff p.[j] %% 16 < 16 by smt().
+      smt().
+qed.
+
+lemma poly_frombytes_poly_tobytes_roundtrip_coeff_range
+    (p : W16.t Array768.t) (j : int) :
+  poly_tobytes_input_qrange p =>
+  0 <= j < 768 =>
+  0 <= coeff (poly_frombytes_spec (poly_tobytes_spec p)).[j] < q.
+proof.
+  move=> Hp Hj.
+  rewrite poly_frombytes_poly_tobytes_roundtrip 1:/#.
+  have Hcoeff :
+      coeff (poly_tobytes_canonical_spec p).[j] = canonical_coeff p.[j]
+    by exact (poly_tobytes_canonical_spec_coeff p j Hp Hj).
+  rewrite Hcoeff.
+  exact (poly_tobytes_canonical_coeff_range p j Hp Hj).
+qed.
+
+lemma poly_frombytes_poly_tobytes_roundtrip_coeff_mod_q
+    (p : W16.t Array768.t) (j : int) :
+  poly_tobytes_input_qrange p =>
+  0 <= j < 768 =>
+  coeff (poly_frombytes_spec (poly_tobytes_spec p)).[j] %% q =
+    coeff p.[j] %% q.
+proof.
+  move=> Hp Hj.
+  rewrite poly_frombytes_poly_tobytes_roundtrip 1:/#.
+  have Hcoeff :
+      coeff (poly_tobytes_canonical_spec p).[j] = canonical_coeff p.[j]
+    by exact (poly_tobytes_canonical_spec_coeff p j Hp Hj).
+  rewrite Hcoeff.
+  exact (canonical_coeff_mod_q p.[j] (Hp j Hj)).
+qed.
+
+lemma poly_tobytes_roundtrip_functional
+    (rp0 : W8.t Array1152.t) (p : W16.t Array768.t) :
+  poly_tobytes_input_qrange p =>
+  hoare [NTRUPlus768PolyToBytes.M.jade_ntruplus_ntruplus768_amd64_ref_poly_tobytes :
+    rp = rp0 /\ ap = p ==>
+    poly_frombytes_spec res = poly_tobytes_canonical_spec p].
+proof.
+  move=> Hp.
+  have Hprocedure_range :
+      NTRUPlus768PolyToBytesProof.poly_tobytes_input_qrange p.
+  + rewrite poly_tobytes_procedure_input_qrangeE.
+    exact Hp.
+  conseq
+    (NTRUPlus768PolyToBytesProof.poly_tobytes_functional
+      rp0 p Hprocedure_range) => /> &hr Hres.
+  rewrite Hres poly_tobytes_procedure_specE.
+  exact (poly_frombytes_poly_tobytes_roundtrip p Hp).
+qed.
+
+lemma poly_tobytes_roundtrip_correct
+    (rp0 : W8.t Array1152.t) (p : W16.t Array768.t) :
+  poly_tobytes_input_qrange p =>
+  phoare [NTRUPlus768PolyToBytes.M.jade_ntruplus_ntruplus768_amd64_ref_poly_tobytes :
+    rp = rp0 /\ ap = p ==>
+    poly_frombytes_spec res = poly_tobytes_canonical_spec p] = 1%r.
+proof.
+  move=> Hp.
+  have Hfunctional := poly_tobytes_roundtrip_functional rp0 p Hp.
+  by conseq NTRUPlus768PolyToBytesProof.poly_tobytes_lossless Hfunctional.
+qed.
