ntruplus/proof/768/ref/poly_tobytes/NTRUPlus768PolyToBytesProof.ec
@@ -1,0 +1,478 @@
+require import AllCore IntDiv Distr Ring StdOrder.
+from Jasmin require import JWord JModel_x86.
+
+require import Array768 Array1152 NTRUPlus768PolyToBytes.
+require import NTRUPlus768BasemulAlgebra.
+require import JWord_extra.
+
+import Ring.IntID IntOrder.
+
+op poly_tobytes_input_qrange (ap : W16.t Array768.t) : bool =
+  forall j, 0 <= j < 768 => -q <= coeff ap.[j] < q.
+
+op canonical_coeff (w : W16.t) : int =
+  if coeff w < 0 then coeff w + q else coeff w.
+
+op poly_tobytes_byte0_int (ap : W16.t Array768.t) (i : int) : int =
+  canonical_coeff ap.[2 * i] %% 256.
+
+op poly_tobytes_byte1_int (ap : W16.t Array768.t) (i : int) : int =
+  canonical_coeff ap.[2 * i] %/ 256 + 16 * (canonical_coeff ap.[2 * i + 1] %% 16).
+
+op poly_tobytes_byte2_int (ap : W16.t Array768.t) (i : int) : int =
+  canonical_coeff ap.[2 * i + 1] %/ 16.
+
+op poly_tobytes_byte_at (ap : W16.t Array768.t) (j : int) : W8.t =
+  if j %% 3 = 0 then
+    W8.of_int (poly_tobytes_byte0_int ap (j %/ 3))
+  else if j %% 3 = 1 then
+    W8.of_int (poly_tobytes_byte1_int ap (j %/ 3))
+  else
+    W8.of_int (poly_tobytes_byte2_int ap (j %/ 3)).
+
+op poly_tobytes_spec (ap : W16.t Array768.t) : W8.t Array1152.t =
+  Array1152.init (fun j => poly_tobytes_byte_at ap j).
+
+op poly_tobytes_canonical_word (w : W16.t) : W16.t =
+  w + ((w `|>>` W8.of_int 15) `&` W16.of_int q).
+
+op poly_tobytes_prefix
+    (ap : W16.t Array768.t) (rp : W8.t Array1152.t) (upto : int) : bool =
+  forall i, 0 <= i < upto =>
+    rp.[3 * i] = W8.of_int (poly_tobytes_byte0_int ap i) /\
+    rp.[3 * i + 1] = W8.of_int (poly_tobytes_byte1_int ap i) /\
+    rp.[3 * i + 2] = W8.of_int (poly_tobytes_byte2_int ap i).
+
+lemma canonical_coeff_range (w : W16.t) :
+  -q <= coeff w < q =>
+  0 <= canonical_coeff w < q.
+proof.
+  move=> Hw.
+  rewrite /canonical_coeff.
+  case (coeff w < 0).
+  + move=> Hneg.
+    rewrite /q /=.
+    smt().
+  move=> Hnonneg.
+  rewrite /q /=.
+  smt().
+qed.
+
+lemma poly_tobytes_W16_of_int_mone :
+  W16.of_int (-1) = W16.onew.
+proof.
+  apply W16.to_uint_eq.
+  rewrite W16.of_uintK W16.to_uint_onew /=.
+  done.
+qed.
+
+lemma poly_tobytes_W16_of_sintK (w : W16.t) :
+  W16.of_int (W16.to_sint w) = w.
+proof.
+  apply W16.to_uint_eq.
+  rewrite W16.of_uintK W16.to_sintE /W16.smod.
+  case (2 ^ (16 - 1) <= W16.to_uint w) => Hsign.
+  + rewrite (modz_sub_dvd
+      (W16.to_uint w) W16.modulus W16.modulus).
+    - by rewrite modzz.
+    by rewrite W16.to_uint_mod.
+  by rewrite W16.to_uint_mod.
+qed.
+
+lemma poly_tobytes_word_from_coeff (w : W16.t) :
+  w = W16.of_int (coeff w).
+proof. by rewrite /coeff poly_tobytes_W16_of_sintK. qed.
+
+lemma poly_tobytes_W16_min_sint_value : W16.min_sint = -32768 by done.
+lemma poly_tobytes_W16_max_sint_value : W16.max_sint = 32767 by done.
+
+lemma poly_tobytes_sign_mask_of_int (x : int) :
+  W16.min_sint <= x <= W16.max_sint =>
+  ((W16.of_int x `|>>` W8.of_int 15) `&` W16.of_int q) =
+  W16.of_int (if x < 0 then q else 0).
+proof.
+  move=> Hx.
+  rewrite poly_tobytes_W16_min_sint_value
+    poly_tobytes_W16_max_sint_value in Hx.
+  have Hcoeff :
+      coeff (W16.of_int x `|>>` W8.of_int 15) = x %/ 2 ^ 15.
+  + rewrite /coeff W16_sar_div 1:/#.
+    rewrite (W16.to_sintK_small x Hx).
+    done.
+  case (x < 0) => Hsign.
+  + rewrite (poly_tobytes_word_from_coeff
+      (W16.of_int x `|>>` W8.of_int 15)).
+    have Hdiv : x %/ 2 ^ 15 = -1.
+    + have Hmin : -32768 <= x by smt().
+      have Hmax : x <= 32767 by smt().
+      have Hpos : 0 < -x by smt().
+      have Hbound : -x <= 32768 by smt().
+      rewrite (_ : x = -(-x)) 1:/#.
+      rewrite divNz 1:Hpos 1:/#.
+      rewrite divz_small; smt().
+    rewrite Hcoeff Hdiv /=.
+    by rewrite poly_tobytes_W16_of_int_mone W16.andwC W16.andw1.
+  rewrite (poly_tobytes_word_from_coeff
+      (W16.of_int x `|>>` W8.of_int 15)).
+  have Hdiv : x %/ 2 ^ 15 = 0.
+  + rewrite divz_small; smt().
+  rewrite Hcoeff Hdiv /=.
+  done.
+qed.
+
+lemma poly_tobytes_canonical_wordE (w : W16.t) :
+  -q <= coeff w < q =>
+  poly_tobytes_canonical_word w = W16.of_int (canonical_coeff w).
+proof.
+  move=> Hw.
+  rewrite /poly_tobytes_canonical_word
+    (poly_tobytes_word_from_coeff w).
+  have Hword : W16.min_sint <= coeff w <= W16.max_sint.
+  + rewrite /q /= in Hw.
+    smt().
+  rewrite (poly_tobytes_sign_mask_of_int (coeff w) Hword).
+  have HcoeffK : coeff (W16.of_int (coeff w)) = coeff w.
+  + rewrite /coeff W16.to_sintK_small 1:Hword.
+    done.
+  rewrite /canonical_coeff HcoeffK.
+  case (coeff w < 0) => Hsign.
+  + by rewrite W16.of_intD.
+  done.
+qed.
+
+lemma poly_tobytes_byte0_wordE (w : W16.t) :
+  -q <= coeff w < q =>
+  truncateu8 (poly_tobytes_canonical_word w) =
+  W8.of_int (canonical_coeff w %% 256).
+proof.
+  move=> Hw.
+  rewrite (poly_tobytes_canonical_wordE w Hw).
+  apply W8.to_uint_eq.
+  rewrite /truncateu8 /= !of_uintK /=.
+  have Hrange := canonical_coeff_range w Hw.
+  rewrite /q /= in Hrange.
+  smt().
+qed.
+
+lemma poly_tobytes_byte2_wordE (w : W16.t) :
+  -q <= coeff w < q =>
+  truncateu8 (poly_tobytes_canonical_word w `>>` W8.of_int 4) =
+  W8.of_int (canonical_coeff w %/ 16).
+proof.
+  move=> Hw.
+  rewrite (poly_tobytes_canonical_wordE w Hw).
+  apply W8.to_uint_eq.
+  rewrite /truncateu8 /= W16.to_uint_shr 1:/# !of_uintK /=.
+  have Hrange := canonical_coeff_range w Hw.
+  rewrite /q /= in Hrange.
+  smt().
+qed.
+
+lemma poly_tobytes_byte1_wordE (w0 w1 : W16.t) :
+  -q <= coeff w0 < q =>
+  -q <= coeff w1 < q =>
+  truncateu8
+    ((poly_tobytes_canonical_word w0 `>>` W8.of_int 8) `|`
+     (poly_tobytes_canonical_word w1 `<<` W8.of_int 4)) =
+  W8.of_int
+    (canonical_coeff w0 %/ 256 + 16 * (canonical_coeff w1 %% 16)).
+proof.
+  move=> Hw0 Hw1.
+  rewrite (poly_tobytes_canonical_wordE w0 Hw0)
+    (poly_tobytes_canonical_wordE w1 Hw1).
+  have Hr0 := canonical_coeff_range w0 Hw0.
+  have Hr1 := canonical_coeff_range w1 Hw1.
+  rewrite /q /= in Hr0.
+  rewrite /q /= in Hr1.
+  rewrite W16.orw_disjoint.
+  + rewrite /W16.(`&`).
+    apply W16.ext_eq => k Hk.
+    rewrite !map2iE // zerowE /(`>>`) /(`<<`) /=.
+    case (k < 4).
+    + smt(W16.get_out).
+    move=> Hk4.
+    rewrite !get_to_uint !of_uintK /=.
+    have Hdiv : canonical_coeff w0 %/ 2 ^ (k + 8) = 0.
+    + apply divz_small.
+      rewrite /CoreInt.absz.
+      have -> : 0 <= 2 ^ (k + 8) by smt(gt0_pow2).
+      rewrite /=.
+      have Hbase : 1 <= 2 by smt().
+      move: (StdOrder.IntOrder.ler_weexpn2l 2 Hbase 12 (k + 8)).
+      move=> Hmono.
+      have Hpow : 2 ^ 12 <= 2 ^ (k + 8).
+      + apply Hmono.
+        smt().
+      have HpowE : 4096 <= 2 ^ (k + 8).
+      + move: Hpow.
+        rewrite (_ : 2 ^ 12 = 4096) 1:/#.
+        done.
+      smt().
+    have Hmod : canonical_coeff w0 %% 65536 = canonical_coeff w0.
+    + rewrite modz_small; smt().
+    rewrite Hmod Hdiv.
+    done.
+  apply W8.to_uint_eq.
+  rewrite /truncateu8 /= W16.to_uintD_small.
+  + rewrite W16.to_uint_shr 1:/# W16.to_uint_shl 1:/#
+      !of_uintK /=.
+    smt().
+  rewrite W16.to_uint_shr 1:/# W16.to_uint_shl 1:/#
+    !of_uintK /=.
+  smt().
+qed.
+
+lemma poly_tobytes_index2E (i : W64.t) :
+  W64.to_uint i < 384 =>
+  W64.to_uint (W64.of_int 2 * i) = 2 * W64.to_uint i.
+proof.
+  move=> Hi.
+  rewrite W64.to_uintM_small.
+  + rewrite W64.of_uintK /=.
+    smt(W64.to_uint_cmp).
+  by rewrite W64.of_uintK /=.
+qed.
+
+lemma poly_tobytes_index2_add1E (i : W64.t) :
+  W64.to_uint i < 384 =>
+  W64.to_uint (W64.of_int 2 * i + W64.one) =
+  2 * W64.to_uint i + 1.
+proof.
+  move=> Hi.
+  rewrite W64.to_uintD_small.
+  + rewrite poly_tobytes_index2E 1:Hi /=.
+    smt(W64.to_uint_cmp).
+  by rewrite poly_tobytes_index2E 1:Hi /=.
+qed.
+
+lemma poly_tobytes_offset3E (i : W64.t) :
+  W64.to_uint i < 384 =>
+  W64.to_uint ((i `<<` W8.one) + i) = 3 * W64.to_uint i.
+proof.
+  move=> Hi.
+  rewrite W64.to_uintD_small.
+  + rewrite /W64.(`<<`) W64.to_uint_shl 1:/# /=.
+    smt(W64.to_uint_cmp).
+  rewrite /W64.(`<<`) W64.to_uint_shl 1:/# /=.
+  rewrite modz_small; first smt(W64.to_uint_cmp).
+  smt().
+qed.
+
+lemma poly_tobytes_offset3_addE (i : W64.t) (d : int) :
+  W64.to_uint i < 384 =>
+  0 <= d <= 2 =>
+  W64.to_uint ((i `<<` W8.one) + i + W64.of_int d) =
+  3 * W64.to_uint i + d.
+proof.
+  move=> Hi Hd.
+  rewrite W64.to_uintD_small.
+  + rewrite poly_tobytes_offset3E 1:Hi W64.of_uintK.
+    rewrite modz_small; smt(W64.to_uint_cmp).
+  rewrite poly_tobytes_offset3E 1:Hi W64.of_uintK.
+  rewrite modz_small; smt(W64.to_uint_cmp).
+qed.
+
+lemma poly_tobytes_byte0_range (ap : W16.t Array768.t) (i : int) :
+  poly_tobytes_input_qrange ap =>
+  0 <= i < 384 =>
+  0 <= poly_tobytes_byte0_int ap i < 256.
+proof.
+  move=> Hap Hi.
+  have Hcanon := canonical_coeff_range ap.[2 * i] _.
+  + apply Hap.
+    smt().
+  rewrite /poly_tobytes_byte0_int.
+  smt().
+qed.
+
+lemma poly_tobytes_byte1_range (ap : W16.t Array768.t) (i : int) :
+  poly_tobytes_input_qrange ap =>
+  0 <= i < 384 =>
+  0 <= poly_tobytes_byte1_int ap i < 256.
+proof.
+  move=> Hap Hi.
+  have Hc0 := canonical_coeff_range ap.[2 * i] _.
+  + apply Hap.
+    smt().
+  have Hc1 := canonical_coeff_range ap.[2 * i + 1] _.
+  + apply Hap.
+    smt().
+  rewrite /poly_tobytes_byte1_int.
+  have Hdiv : 0 <= canonical_coeff ap.[2 * i] %/ 256 < 16 by smt().
+  have Hmod : 0 <= canonical_coeff ap.[2 * i + 1] %% 16 < 16 by smt().
+  smt().
+qed.
+
+lemma poly_tobytes_byte2_range (ap : W16.t Array768.t) (i : int) :
+  poly_tobytes_input_qrange ap =>
+  0 <= i < 384 =>
+  0 <= poly_tobytes_byte2_int ap i < 256.
+proof.
+  move=> Hap Hi.
+  have Hcanon := canonical_coeff_range ap.[2 * i + 1] _.
+  + apply Hap.
+    smt().
+  rewrite /poly_tobytes_byte2_int.
+  smt().
+qed.
+
+lemma poly_tobytes_prefix_extend
+    (ap : W16.t Array768.t) (rp : W8.t Array1152.t) (i : int) :
+  poly_tobytes_input_qrange ap =>
+  0 <= i < 384 =>
+  poly_tobytes_prefix ap rp i =>
+  poly_tobytes_prefix ap
+    (rp.[3 * i <- W8.of_int (poly_tobytes_byte0_int ap i)]
+       .[3 * i + 1 <- W8.of_int (poly_tobytes_byte1_int ap i)]
+       .[3 * i + 2 <- W8.of_int (poly_tobytes_byte2_int ap i)]) (i + 1).
+proof.
+  move=> Hap Hi Hprefix j Hj.
+  case (j = i) => [-> | Hneq].
+  + smt(Array1152.get_setE).
+  have Hjold : 0 <= j < i by smt().
+  have Hold := Hprefix j Hjold.
+  move: Hold => [H0 [H1 H2]].
+  smt(Array1152.get_setE).
+qed.
+
+lemma poly_tobytes_spec_byte0E (ap : W16.t Array768.t) (i : int) :
+  0 <= i < 384 =>
+  (poly_tobytes_spec ap).[3 * i] = W8.of_int (poly_tobytes_byte0_int ap i).
+proof.
+  move=> Hi.
+  rewrite /poly_tobytes_spec Array1152.initiE 1:/# /poly_tobytes_byte_at.
+  smt().
+qed.
+
+lemma poly_tobytes_spec_byte1E (ap : W16.t Array768.t) (i : int) :
+  0 <= i < 384 =>
+  (poly_tobytes_spec ap).[3 * i + 1] = W8.of_int (poly_tobytes_byte1_int ap i).
+proof.
+  move=> Hi.
+  rewrite /poly_tobytes_spec Array1152.initiE 1:/# /poly_tobytes_byte_at.
+  smt().
+qed.
+
+lemma poly_tobytes_spec_byte2E (ap : W16.t Array768.t) (i : int) :
+  0 <= i < 384 =>
+  (poly_tobytes_spec ap).[3 * i + 2] = W8.of_int (poly_tobytes_byte2_int ap i).
+proof.
+  move=> Hi.
+  rewrite /poly_tobytes_spec Array1152.initiE 1:/# /poly_tobytes_byte_at.
+  smt().
+qed.
+
+lemma poly_tobytes_prefix_full
+    (ap : W16.t Array768.t) (rp : W8.t Array1152.t) :
+  poly_tobytes_prefix ap rp 384 =>
+  rp = poly_tobytes_spec ap.
+proof.
+  move=> Hprefix.
+  apply Array1152.tP => j Hj.
+  have Hjpair : 0 <= j %/ 3 < 384 by smt().
+  move: (Hprefix (j %/ 3) Hjpair) => [H0 [H1 H2]].
+  case (j %% 3 = 0).
+  + move=> Hmod.
+    have -> : j = 3 * (j %/ 3) by smt().
+    rewrite H0.
+    by rewrite (poly_tobytes_spec_byte0E ap (j %/ 3) Hjpair).
+  case (j %% 3 = 1).
+  + move=> Hmod0 Hmod1.
+    have -> : j = 3 * (j %/ 3) + 1 by smt().
+    rewrite H1.
+    by rewrite (poly_tobytes_spec_byte1E ap (j %/ 3) Hjpair).
+  move=> Hmod0 Hmod1.
+  have -> : j = 3 * (j %/ 3) + 2 by smt().
+  rewrite H2.
+  by rewrite (poly_tobytes_spec_byte2E ap (j %/ 3) Hjpair).
+qed.
+
+lemma poly_tobytes_functional
+    (rp0 : W8.t Array1152.t) (ap0 : W16.t Array768.t) :
+  poly_tobytes_input_qrange ap0 =>
+  hoare [NTRUPlus768PolyToBytes.M.jade_ntruplus_ntruplus768_amd64_ref_poly_tobytes :
+    rp = rp0 /\ ap = ap0 ==>
+    res = poly_tobytes_spec ap0].
+proof.
+  move=> Hap0.
+  proc.
+  seq 2 :
+    (ap = ap0 /\ i = W64.of_int 0 /\ poly_tobytes_prefix ap0 rp 0).
+  + auto => />.
+    rewrite /poly_tobytes_prefix.
+    smt().
+  while (0 <= W64.to_uint i <= 384 /\ ap = ap0 /\
+         poly_tobytes_prefix ap0 rp (W64.to_uint i)); last first.
+  + skip => &hr [Hap [Hi0 Hprefix0]].
+    split.
+    - split; first by rewrite Hi0 W64.to_uint0; smt().
+      split; first exact Hap.
+      by rewrite Hi0 W64.to_uint0.
+    move=> i1 rp1 Hexit [Hi [Hap1 Hprefix1]].
+    rewrite W64.ultE /= in Hexit.
+    apply poly_tobytes_prefix_full.
+    have Hiend : W64.to_uint i1 = 384 by smt().
+    by rewrite -Hiend.
+  auto => /> &hr HiLow HiHigh Hprefix Hloop.
+  rewrite W64.ultE /= in Hloop.
+  have Hi384 : 0 <= W64.to_uint i{hr} < 384 by smt().
+  have HiLt : W64.to_uint i{hr} < 384 by smt().
+  have Hnext :
+      W64.to_uint (i{hr} + W64.one) =
+      W64.to_uint i{hr} + 1.
+  + rewrite W64.to_uintD_small /=; smt(W64.to_uint_cmp).
+  split.
+  + rewrite Hnext; smt(W64.to_uint_cmp).
+  have Heven :
+      -q <= coeff ap0.[2 * W64.to_uint i{hr}] < q.
+  + apply Hap0.
+    smt().
+  have Hodd :
+      -q <= coeff ap0.[2 * W64.to_uint i{hr} + 1] < q.
+  + apply Hap0.
+    smt().
+  rewrite Hnext.
+  rewrite (poly_tobytes_offset3E i{hr} HiLt).
+  rewrite (poly_tobytes_offset3_addE i{hr} 1 HiLt _) 1:/#.
+  rewrite (poly_tobytes_offset3_addE i{hr} 2 HiLt _) 1:/#.
+  rewrite (poly_tobytes_index2E i{hr} HiLt).
+  rewrite (poly_tobytes_index2_add1E i{hr} HiLt).
+  rewrite -/poly_tobytes_canonical_word.
+  rewrite (poly_tobytes_byte0_wordE
+      ap0.[2 * W64.to_uint i{hr}] Heven).
+  rewrite (poly_tobytes_byte1_wordE
+      ap0.[2 * W64.to_uint i{hr}]
+      ap0.[2 * W64.to_uint i{hr} + 1] Heven Hodd).
+  rewrite (poly_tobytes_byte2_wordE
+      ap0.[2 * W64.to_uint i{hr} + 1] Hodd).
+  rewrite -/poly_tobytes_byte0_int -/poly_tobytes_byte1_int
+    -/poly_tobytes_byte2_int.
+  apply poly_tobytes_prefix_extend; first exact Hap0.
+  + exact Hi384.
+  exact Hprefix.
+qed.
+
+lemma poly_tobytes_lossless :
+  islossless
+    NTRUPlus768PolyToBytes.M.jade_ntruplus_ntruplus768_amd64_ref_poly_tobytes.
+proof.
+  proc.
+  while (0 <= W64.to_uint i <= 384) (384 - W64.to_uint i); last first.
+  + auto => /> i0 Hi Hdone.
+    rewrite W64.ultE /=.
+    smt().
+  auto => /> &hr Hi Hhigh Hloop.
+  rewrite W64.ultE /= in Hloop.
+  rewrite W64.to_uintD_small /=; smt(W64.to_uint_cmp).
+qed.
+
+lemma poly_tobytes_correct
+    (rp0 : W8.t Array1152.t) (ap0 : W16.t Array768.t) :
+  poly_tobytes_input_qrange ap0 =>
+  phoare [NTRUPlus768PolyToBytes.M.jade_ntruplus_ntruplus768_amd64_ref_poly_tobytes :
+    rp = rp0 /\ ap = ap0 ==>
+    res = poly_tobytes_spec ap0] = 1%r.
+proof.
+  move=> Hap0.
+  by conseq poly_tobytes_lossless (poly_tobytes_functional rp0 ap0 Hap0).
+qed.
