ntruplus/proof/768/ref/poly_tobytes/extracted/NTRUPlus768PolyToBytes.ec
@@ -1,0 +1,50 @@
+require import AllCore IntDiv CoreMap List Distr.
+
+from Jasmin require import JModel_x86.
+
+import SLH64.
+
+require import Array768 Array1152 WArray1152 WArray1536.
+
+module M = {
+  proc jade_ntruplus_ntruplus768_amd64_ref_poly_tobytes (rp:W8.t Array1152.t,
+                                                         ap:W16.t Array768.t) :
+  W8.t Array1152.t = {
+    var i:W64.t;
+    var off:W64.t;
+    var t0:W16.t;
+    var mask:W16.t;
+    var t1:W16.t;
+    var t:W16.t;
+    var  _0:W64.t;
+     _0 <- (init_msf);
+    i <- (W64.of_int 0);
+    while ((i \ult (W64.of_int (768 %/ 2)))) {
+      off <- i;
+      off <- (off `<<` (W8.of_int 1));
+      t0 <- ap.[(W64.to_uint ((W64.of_int 2) * i))];
+      mask <- t0;
+      mask <- (mask `|>>` (W8.of_int 15));
+      mask <- (mask `&` (W16.of_int 3457));
+      t0 <- (t0 + mask);
+      t1 <- ap.[(W64.to_uint (((W64.of_int 2) * i) + (W64.of_int 1)))];
+      mask <- t1;
+      mask <- (mask `|>>` (W8.of_int 15));
+      mask <- (mask `&` (W16.of_int 3457));
+      t1 <- (t1 + mask);
+      off <- (off + i);
+      rp.[(W64.to_uint off)] <- (truncateu8 t0);
+      t <- t0;
+      t <- (t `>>` (W8.of_int 8));
+      mask <- t1;
+      mask <- (mask `<<` (W8.of_int 4));
+      t <- (t `|` mask);
+      rp.[(W64.to_uint (off + (W64.of_int 1)))] <- (truncateu8 t);
+      t <- t1;
+      t <- (t `>>` (W8.of_int 4));
+      rp.[(W64.to_uint (off + (W64.of_int 2)))] <- (truncateu8 t);
+      i <- (i + (W64.of_int 1));
+    }
+    return rp;
+  }
+}.
